code/k256/Hacl.Impl.K256.PrecompTable.fst
@@ -1,0 +1,575 @@
+module Hacl.Impl.K256.PrecompTable
+
+open FStar.Mul
+open Lib.IntTypes
+open Lib.Sequence
+
+open Hacl.Spec.K256.Field52.Definitions
+open Hacl.Impl.K256.Point
+
+module S = Spec.K256
+module SL = Spec.K256.Lemmas
+
+module LE = Lib.Exponentiation
+module SE = Spec.Exponentiation
+
+#set-options "--z3rlimit 50 --fuel 0 --ifuel 0"
+
+// unfold let precomp_basepoint_table_list: list uint64 = [
+//   // P_0
+//   u64 0x0; u64 0x0; u64 0x0; u64 0x0; u64 0x0;
+//   u64 0x1; u64 0x0; u64 0x0; u64 0x0; u64 0x0;
+//   u64 0x0; u64 0x0; u64 0x0; u64 0x0; u64 0x0;
+//   // P_1
+//   u64 0x2815b16f81798; u64 0xdb2dce28d959f; u64 0xe870b07029bfc; u64 0xbbac55a06295c; u64 0x79be667ef9dc;
+//   u64 0x7d08ffb10d4b8; u64 0x48a68554199c4; u64 0xe1108a8fd17b4; u64 0xc4655da4fbfc0; u64 0x483ada7726a3;
+//   u64 0x1; u64 0x0; u64 0x0; u64 0x0; u64 0x0;
+//   // P_2
+//   u64 0x48e044f109fc8; u64 0x373c920774523; u64 0x39ac4b67827eb; u64 0xf9aa5402b9fdc; u64 0xf40af3b6c6fd;
+//   u64 0x89164bfadcbdb; u64 0x3e1b1383f85fe; u64 0xf60db4a43bf63; u64 0xc8f76f5fd7e4b; u64 0x56915849f52c;
+//   u64 0x6ba5554759a29; u64 0xcdc3eac498b0c; u64 0x31fc97023dc71; u64 0xa307b568a6ad9; u64 0xf8783c53dfb2;
+//   // P_3
+//   u64 0x743bb790f36b0; u64 0x85fc6b4b9f2d4; u64 0xca8a1c32e8a3a; u64 0x8a2cf6a7671fe; u64 0x60cf61741984;
+//   u64 0x7ed686f22d3a4; u64 0xcf01cb6ba7740; u64 0x49580fb29f8d; u64 0x802c4496c6c94; u64 0x884936b7356d;
+//   u64 0x8300925d6f1d4; u64 0x890c0c39e497e; u64 0x9a33c7290e5dc; u64 0x8ab5595351ab8; u64 0x5ac0eb0fb539;
+//   // P_4
+//   u64 0xa8d95e8d08c8; u64 0x424d85dec433d; u64 0xf04fa8fc34e5f; u64 0x14139cb1bf9c7; u64 0x1d743fca4032;
+//   u64 0xa9845fe3f605e; u64 0x91fde09e494b2; u64 0xc472eb4ef7b21; u64 0xc0fbe29ead4d6; u64 0x34fb8147eed1;
+//   u64 0xac2271100e68d; u64 0x9984e7e4edd6c; u64 0xe67898df910fc; u64 0x1b2c871f6070c; u64 0x81554cf0ba11;
+//   // P_5
+//   u64 0x7589553034c8c; u64 0xfae143ee6bbd1; u64 0xd2a4dddf72bef; u64 0xf808e1673167d; u64 0x6c31fec38a52;
+//   u64 0x415c48ab514d1; u64 0xdd5a8fe6960a; u64 0xcb851560de31c; u64 0xcda57740c3eea; u64 0x995d6e0c6c03;
+//   u64 0x3730d5ce6c85d; u64 0x55d61f66e6306; u64 0x4689c998a59d8; u64 0x3ba10c0c653d9; u64 0x5e87c80e6ebc;
+//   // P_6
+//   u64 0x3b372eb0f81b5; u64 0x8c759d6268fd4; u64 0xb319ed808b9fd; u64 0x38de42e3e7b13; u64 0x500e998c69da;
+//   u64 0x701bb58f3bf9b; u64 0x8bfa9947ce5e6; u64 0x9db75c5e83c22; u64 0x991e8c18d4a68; u64 0x85bbc16d25ec;
+//   u64 0x9e679560f6767; u64 0xc878c8474b933; u64 0xcf7ac54533c20; u64 0xef22f54742509; u64 0x6f7961ae1d9d;
+//   // P_7
+//   u64 0x92852b11abe5a; u64 0x4f646416eae4e; u64 0xb639adaa34214; u64 0x18f4c410d3a43; u64 0x10d5ba07117f;
+//   u64 0x5ccc4d5223f0c; u64 0x5348c992c9e65; u64 0x9dc603dd22c90; u64 0x5fd882ef1ff18; u64 0x740429e4bdfd;
+//   u64 0x49213a87245d0; u64 0x1f235d735b13c; u64 0x5a56659b7d254; u64 0xd6f6f7b4a5eb; u64 0xa1ea9d796daf;
+//   // P_8
+//   u64 0xd354595e8091c; u64 0x59727a946d712; u64 0x1ad2fd6b09d6c; u64 0xc18040ba67527; u64 0x94e6b56ba0ec;
+//   u64 0x80fcb21037704; u64 0x665a87a06743f; u64 0x1cbeb09af2bf3; u64 0x9d72fe7feb032; u64 0xb74df0c21371;
+//   u64 0xb17d5ffe6d714; u64 0x1e355dee022fd; u64 0xac21796140533; u64 0xb639a93da6f3d; u64 0xe15a35015997;
+//   // P_9
+//   u64 0xb9c5b6ef1f43b; u64 0x2a7bc283fc49f; u64 0x88e368394993f; u64 0xed7b8a9e60d3d; u64 0xf721d2dad6f6;
+//   u64 0xec454b7860999; u64 0x89673b944d8e0; u64 0x309522ce23a1a; u64 0x5193173cc4dd9; u64 0x9a1facd6b25a;
+//   u64 0xad69b0614f7a2; u64 0xb8d1b10c02e19; u64 0xbc2a2c7b66ffb; u64 0xee4bdc91b3aa8; u64 0xa2b275bde29d;
+//   // P_10
+//   u64 0x31ac94b24208e; u64 0x11aeaf4ece6d; u64 0xa413faa8d7937; u64 0x90d8df1df29ff; u64 0x5f8d622d2557;
+//   u64 0x592ce6949080d; u64 0xf125a05cefe03; u64 0x6d0aa60d51e9b; u64 0x4f07f7c3cf9d4; u64 0x4af6e1ccf133;
+//   u64 0xf0f95a3be72b8; u64 0xd3f6d52e63a92; u64 0x17d9ecbe226d1; u64 0x6b6af333c989a; u64 0xe625b11d9a14;
+//   // P_11
+//   u64 0xd154f79d8e341; u64 0x7cc8bb59c85ee; u64 0xa13927fe452be; u64 0x6e08fbee3b; u64 0xd24d031b1185;
+//   u64 0x5c715d4620a0b; u64 0xaa5fd2660d143; u64 0x66bc46a0d83d0; u64 0x2c519acec26ae; u64 0x6c3b82462505;
+//   u64 0x8b8cbd971ab15; u64 0xe8501868aee69; u64 0xc54addf1d50d; u64 0x4d8da1ea82014; u64 0x56e000de4c56;
+//   // P_12
+//   u64 0xbc3731f4e710b; u64 0xf5fe753395cd; u64 0x2804f4c0bc49f; u64 0x11ae10debc618; u64 0x4f17b524159f;
+//   u64 0xaae89f1f9385d; u64 0x856a1901e3aea; u64 0x2d28d08cc0cec; u64 0x93d8d337da9b; u64 0x5feedb5497d3;
+//   u64 0x5d06206f529e1; u64 0x6c479715a827a; u64 0x48a2dd96d0f48; u64 0x3fdeb0c237630; u64 0x1db55c9d4eaa;
+//   // P_13
+//   u64 0xe0696573c7533; u64 0x63e4658737869; u64 0x2a11f253f4b05; u64 0x229a7e15cdf48; u64 0x3b9f32f54a4f;
+//   u64 0x327e4ceccc2ba; u64 0x3e26d2be9d0df; u64 0x82a00f70af042; u64 0x6020d484c25d6; u64 0xe839a854faeb;
+//   u64 0x21ded5312b490; u64 0xf1b776c83d9ed; u64 0x41f6a2c735d44; u64 0x7adcc8a05f3b5; u64 0xd926fe353140;
+//   // P_14
+//   u64 0xc2b376c728ec; u64 0x947782c52046f; u64 0x27ba54a224d00; u64 0x1035e99c0bf5e; u64 0x612ca1b20e84;
+//   u64 0x789d7d062632e; u64 0x683f45cb279ba; u64 0x8b8fac6a007b2; u64 0x350c84e93fa4; u64 0x18a55aa52df;
+//   u64 0xe94da9625f527; u64 0xd2619ce2f8a88; u64 0x942403888b43e; u64 0x961da5fd1dc90; u64 0x2f1506d7e117;
+//   // P_15
+//   u64 0x34deee761bce2; u64 0xfb484324815cc; u64 0xcd7cc675d3a1d; u64 0xca0691e2a6447; u64 0xbb6b7f7b8fa2;
+//   u64 0x6c53975090d10; u64 0xa14a4124a90d2; u64 0xbb94d4b653242; u64 0x5074f7da14c32; u64 0xec662837477c;
+//   u64 0xee9be37d0b9b; u64 0x4fba9fd90713b; u64 0xcc62c6dc14aa4; u64 0x695bf61db25ac; u64 0x36ba954be769
+// ]
+
+
+unfold
+let create15 (x0 x1 x2 x3 x4 x5 x6 x7 x8 x9 x10 x11 x12 x13 x14:uint64) : list uint64 =
+  [x0; x1; x2; x3; x4; x5; x6; x7; x8; x9; x10; x11; x12; x13; x14]
+
+let create15_lseq (x0 x1 x2 x3 x4 x5 x6 x7 x8 x9 x10 x11 x12 x13 x14:uint64) : lseq uint64 15 =
+  let l = [x0; x1; x2; x3; x4; x5; x6; x7; x8; x9; x10; x11; x12; x13; x14] in
+  assert_norm (List.Tot.length l = 15);
+  Seq.seq_of_list l
+
+val create15_lemma (x0 x1 x2 x3 x4 x5 x6 x7 x8 x9 x10 x11 x12 x13 x14:uint64) :
+  Lemma (let s = create15_lseq x0 x1 x2 x3 x4 x5 x6 x7 x8 x9 x10 x11 x12 x13 x14 in
+    s.[0] == x0 /\ s.[1] == x1 /\ s.[2] == x2 /\ s.[3] == x3 /\
+    s.[4] == x4 /\ s.[5] == x5 /\ s.[6] == x6 /\ s.[7] == x7 /\
+    s.[8] == x8 /\ s.[9] == x9 /\ s.[10] == x10 /\ s.[11] == x11 /\
+    s.[12] == x12 /\ s.[13] == x13 /\ s.[14] == x14)
+
+let create15_lemma x0 x1 x2 x3 x4 x5 x6 x7 x8 x9 x10 x11 x12 x13 x14 =
+  Seq.elim_of_list [x0; x1; x2; x3; x4; x5; x6; x7; x8; x9; x10; x11; x12; x13; x14]
+
+let pow_base_point (k:nat) =
+  LE.pow S.mk_k256_comm_monoid (S.to_aff_point S.g) k
+
+//-----------------------
+
+unfold
+let p0_list : list uint64 =
+  create15
+    (u64 0x0) (u64 0x0) (u64 0x0) (u64 0x0) (u64 0x0)
+    (u64 0x1) (u64 0x0) (u64 0x0) (u64 0x0) (u64 0x0)
+    (u64 0x0) (u64 0x0) (u64 0x0) (u64 0x0) (u64 0x0)
+
+let p0_lseq : lseq uint64 15 =
+  assert_norm (List.Tot.length p0_list = 15);
+  Seq.seq_of_list p0_list
+
+val p0_lemma : unit -> Lemma (point_eval_lseq p0_lseq == S.point_at_inf_c ())
+let p0_lemma () =
+  create15_lemma
+    (u64 0x0) (u64 0x0) (u64 0x0) (u64 0x0) (u64 0x0)
+    (u64 0x1) (u64 0x0) (u64 0x0) (u64 0x0) (u64 0x0)
+    (u64 0x0) (u64 0x0) (u64 0x0) (u64 0x0) (u64 0x0)
+
+val p0_is_pow0_lemma: unit -> Lemma (S.to_aff_point (point_eval_lseq p0_lseq) == pow_base_point 0)
+let p0_is_pow0_lemma () =
+  p0_lemma ();
+  LE.lemma_pow0 S.mk_k256_comm_monoid (S.to_aff_point S.g)
+
+//-----------------------
+
+unfold
+let p1_list : list uint64 =
+  create15
+  (u64 0x2815b16f81798) (u64 0xdb2dce28d959f) (u64 0xe870b07029bfc) (u64 0xbbac55a06295c) (u64 0x79be667ef9dc)
+  (u64 0x7d08ffb10d4b8) (u64 0x48a68554199c4) (u64 0xe1108a8fd17b4) (u64 0xc4655da4fbfc0) (u64 0x483ada7726a3)
+  (u64 0x1) (u64 0x0) (u64 0x0) (u64 0x0) (u64 0x0)
+
+let p1_lseq : lseq uint64 15 =
+  assert_norm (List.Tot.length p1_list = 15);
+  Seq.seq_of_list p1_list
+
+val p1_lemma : unit -> Lemma (point_eval_lseq p1_lseq == S.g)
+let p1_lemma () =
+  create15_lemma
+  (u64 0x2815b16f81798) (u64 0xdb2dce28d959f) (u64 0xe870b07029bfc) (u64 0xbbac55a06295c) (u64 0x79be667ef9dc)
+  (u64 0x7d08ffb10d4b8) (u64 0x48a68554199c4) (u64 0xe1108a8fd17b4) (u64 0xc4655da4fbfc0) (u64 0x483ada7726a3)
+  (u64 0x1) (u64 0x0) (u64 0x0) (u64 0x0) (u64 0x0)
+
+val p1_is_pow1_lemma: unit -> Lemma (S.to_aff_point (point_eval_lseq p1_lseq) == pow_base_point 1)
+let p1_is_pow1_lemma () =
+  p1_lemma ();
+  LE.lemma_pow1 S.mk_k256_comm_monoid (S.to_aff_point S.g)
+
+//-----------------------
+
+unfold
+let p2_list : list uint64 =
+  create15
+    (u64 0x48e044f109fc8) (u64 0x373c920774523) (u64 0x39ac4b67827eb) (u64 0xf9aa5402b9fdc) (u64 0xf40af3b6c6fd)
+    (u64 0x89164bfadcbdb) (u64 0x3e1b1383f85fe) (u64 0xf60db4a43bf63) (u64 0xc8f76f5fd7e4b) (u64 0x56915849f52c)
+    (u64 0x6ba5554759a29) (u64 0xcdc3eac498b0c) (u64 0x31fc97023dc71) (u64 0xa307b568a6ad9) (u64 0xf8783c53dfb2)
+
+let p2_lseq : lseq uint64 15 =
+  assert_norm (List.Tot.length p2_list = 15);
+  Seq.seq_of_list p2_list
+
+val p2_eval_lemma : unit -> Lemma
+  (let x, y, z = point_eval_lseq p2_lseq in
+   let qx = 0xf40af3b6c6fdf9aa5402b9fdc39ac4b67827eb373c92077452348e044f109fc8 in
+   let qy = 0x56915849f52cc8f76f5fd7e4bf60db4a43bf633e1b1383f85fe89164bfadcbdb in
+   let qz = 0xf8783c53dfb2a307b568a6ad931fc97023dc71cdc3eac498b0c6ba5554759a29 in
+   x == qx /\ y == qy /\ z == qz)
+
+let p2_eval_lemma () =
+  create15_lemma
+    (u64 0x48e044f109fc8) (u64 0x373c920774523) (u64 0x39ac4b67827eb) (u64 0xf9aa5402b9fdc) (u64 0xf40af3b6c6fd)
+    (u64 0x89164bfadcbdb) (u64 0x3e1b1383f85fe) (u64 0xf60db4a43bf63) (u64 0xc8f76f5fd7e4b) (u64 0x56915849f52c)
+    (u64 0x6ba5554759a29) (u64 0xcdc3eac498b0c) (u64 0x31fc97023dc71) (u64 0xa307b568a6ad9) (u64 0xf8783c53dfb2)
+
+val p2_lemma : unit -> Lemma (point_eval_lseq p2_lseq == S.point_add S.g S.g)
+let p2_lemma () =
+  let qx = 0xf40af3b6c6fdf9aa5402b9fdc39ac4b67827eb373c92077452348e044f109fc8 in
+  let qy = 0x56915849f52cc8f76f5fd7e4bf60db4a43bf633e1b1383f85fe89164bfadcbdb in
+  let qz = 0xf8783c53dfb2a307b568a6ad931fc97023dc71cdc3eac498b0c6ba5554759a29 in
+  let px, py, pz = normalize_term (S.point_add S.g S.g) in
+  assert (qx == px /\ qy = py /\ qz = pz);
+  p2_eval_lemma ();
+  let x, y, z = point_eval_lseq p2_lseq in
+  assert (x == qx /\ y == qy /\ z == qz);
+  normalize_term_spec (S.point_add S.g S.g);
+  assert ((px, py, pz) == S.point_add S.g S.g);
+  assert (px = x /\ py = y /\ pz = z);
+  assert (point_eval_lseq p2_lseq == S.point_add S.g S.g)
+
+val p2_is_pow2_lemma: unit -> Lemma (S.to_aff_point (point_eval_lseq p2_lseq) == pow_base_point 2)
+let p2_is_pow2_lemma () =
+  let g_aff = S.to_aff_point S.g in
+  p2_lemma ();
+  SL.to_aff_point_add_lemma S.g S.g;
+  assert (S.to_aff_point (point_eval_lseq p2_lseq) == S.aff_point_add g_aff g_aff);
+  LE.lemma_pow_unfold S.mk_k256_comm_monoid g_aff 2;
+  LE.lemma_pow1 S.mk_k256_comm_monoid g_aff;
+  assert (pow_base_point 2 == S.aff_point_add g_aff g_aff)
+
+//-----------------------
+
+unfold
+let p3_list : list uint64 =
+  create15
+  (u64 0x743bb790f36b0) (u64 0x85fc6b4b9f2d4) (u64 0xca8a1c32e8a3a) (u64 0x8a2cf6a7671fe) (u64 0x60cf61741984)
+  (u64 0x7ed686f22d3a4) (u64 0xcf01cb6ba7740) (u64 0x49580fb29f8d) (u64 0x802c4496c6c94) (u64 0x884936b7356d)
+  (u64 0x8300925d6f1d4) (u64 0x890c0c39e497e) (u64 0x9a33c7290e5dc) (u64 0x8ab5595351ab8) (u64 0x5ac0eb0fb539)
+
+let p3_lseq : lseq uint64 15 =
+  assert_norm (List.Tot.length p3_list = 15);
+  Seq.seq_of_list p3_list
+
+val p3_eval_lemma : unit -> Lemma
+  (let x, y, z = point_eval_lseq p3_lseq in
+  let qx = 0x60cf617419848a2cf6a7671feca8a1c32e8a3a85fc6b4b9f2d4743bb790f36b0 in
+  let qy = 0x884936b7356d802c4496c6c94049580fb29f8dcf01cb6ba77407ed686f22d3a4 in
+  let qz = 0x5ac0eb0fb5398ab5595351ab89a33c7290e5dc890c0c39e497e8300925d6f1d4 in
+   x == qx /\ y == qy /\ z == qz)
+
+let p3_eval_lemma () =
+  create15_lemma
+  (u64 0x743bb790f36b0) (u64 0x85fc6b4b9f2d4) (u64 0xca8a1c32e8a3a) (u64 0x8a2cf6a7671fe) (u64 0x60cf61741984)
+  (u64 0x7ed686f22d3a4) (u64 0xcf01cb6ba7740) (u64 0x49580fb29f8d) (u64 0x802c4496c6c94) (u64 0x884936b7356d)
+  (u64 0x8300925d6f1d4) (u64 0x890c0c39e497e) (u64 0x9a33c7290e5dc) (u64 0x8ab5595351ab8) (u64 0x5ac0eb0fb539)
+
+val p3_lemma : unit -> Lemma (point_eval_lseq p3_lseq == S.point_add (point_eval_lseq p2_lseq) S.g)
+let p3_lemma () =
+  let qx = 0x60cf617419848a2cf6a7671feca8a1c32e8a3a85fc6b4b9f2d4743bb790f36b0 in
+  let qy = 0x884936b7356d802c4496c6c94049580fb29f8dcf01cb6ba77407ed686f22d3a4 in
+  let qz = 0x5ac0eb0fb5398ab5595351ab89a33c7290e5dc890c0c39e497e8300925d6f1d4 in
+
+  let rx = 0xf40af3b6c6fdf9aa5402b9fdc39ac4b67827eb373c92077452348e044f109fc8 in
+  let ry = 0x56915849f52cc8f76f5fd7e4bf60db4a43bf633e1b1383f85fe89164bfadcbdb in
+  let rz = 0xf8783c53dfb2a307b568a6ad931fc97023dc71cdc3eac498b0c6ba5554759a29 in
+
+  let px, py, pz = normalize_term (S.point_add (rx, ry, rz) S.g) in
+  assert (qx == px /\ qy = py /\ qz = pz);
+  p2_eval_lemma (); // assert ((rx, ry, rz) == point_eval_lseq p2_lseq);
+  let x, y, z = point_eval_lseq p3_lseq in
+  p3_eval_lemma (); // assert (x == qx /\ y == qy /\ z == qz);
+  normalize_term_spec (S.point_add (rx, ry, rz) S.g);
+  assert ((px, py, pz) == S.point_add (rx, ry, rz) S.g);
+  assert (px = x /\ py = y /\ pz = z);
+  assert (point_eval_lseq p3_lseq == S.point_add (rx, ry, rz) S.g)
+
+val p3_is_pow3_lemma: unit -> Lemma (S.to_aff_point (point_eval_lseq p3_lseq) == pow_base_point 3)
+let p3_is_pow3_lemma () =
+  let g_aff = S.to_aff_point S.g in
+  calc (==) {
+    S.to_aff_point (point_eval_lseq p3_lseq);
+    (==) { p3_lemma () }
+    S.to_aff_point (S.point_add (point_eval_lseq p2_lseq) S.g);
+    (==) { SL.to_aff_point_add_lemma (point_eval_lseq p2_lseq) S.g }
+    S.aff_point_add (S.to_aff_point (point_eval_lseq p2_lseq)) g_aff;
+    (==) { p2_is_pow2_lemma () }
+    S.aff_point_add (pow_base_point 2) g_aff;
+    (==) { LE.lemma_pow1 S.mk_k256_comm_monoid g_aff }
+    S.aff_point_add (pow_base_point 2) (pow_base_point 1);
+    (==) { LE.lemma_pow_add S.mk_k256_comm_monoid g_aff 2 1 }
+    pow_base_point 3;
+  }
+
+//-----------------------
+
+unfold
+let p4_list : list uint64 =
+  create15
+  (u64 0xa8d95e8d08c8) (u64 0x424d85dec433d) (u64 0xf04fa8fc34e5f) (u64 0x14139cb1bf9c7) (u64 0x1d743fca4032)
+  (u64 0xa9845fe3f605e) (u64 0x91fde09e494b2) (u64 0xc472eb4ef7b21) (u64 0xc0fbe29ead4d6) (u64 0x34fb8147eed1)
+  (u64 0xac2271100e68d) (u64 0x9984e7e4edd6c) (u64 0xe67898df910fc) (u64 0x1b2c871f6070c) (u64 0x81554cf0ba11)
+
+let p4_lseq : lseq uint64 15 =
+  assert_norm (List.Tot.length p4_list = 15);
+  Seq.seq_of_list p4_list
+
+assume
+val p4_is_pow4_lemma: unit -> Lemma (S.to_aff_point (point_eval_lseq p4_lseq) == pow_base_point 4)
+
+//-----------------------
+
+unfold
+let p5_list : list uint64 =
+  create15
+  (u64 0x7589553034c8c) (u64 0xfae143ee6bbd1) (u64 0xd2a4dddf72bef) (u64 0xf808e1673167d) (u64 0x6c31fec38a52)
+  (u64 0x415c48ab514d1) (u64 0xdd5a8fe6960a) (u64 0xcb851560de31c) (u64 0xcda57740c3eea) (u64 0x995d6e0c6c03)
+  (u64 0x3730d5ce6c85d) (u64 0x55d61f66e6306) (u64 0x4689c998a59d8) (u64 0x3ba10c0c653d9) (u64 0x5e87c80e6ebc)
+
+let p5_lseq : lseq uint64 15 =
+  assert_norm (List.Tot.length p5_list = 15);
+  Seq.seq_of_list p5_list
+
+assume
+val p5_is_pow5_lemma: unit -> Lemma (S.to_aff_point (point_eval_lseq p5_lseq) == pow_base_point 5)
+
+//-----------------------
+
+unfold
+let p6_list : list uint64 =
+  create15
+  (u64 0x3b372eb0f81b5) (u64 0x8c759d6268fd4) (u64 0xb319ed808b9fd) (u64 0x38de42e3e7b13) (u64 0x500e998c69da)
+  (u64 0x701bb58f3bf9b) (u64 0x8bfa9947ce5e6) (u64 0x9db75c5e83c22) (u64 0x991e8c18d4a68) (u64 0x85bbc16d25ec)
+  (u64 0x9e679560f6767) (u64 0xc878c8474b933) (u64 0xcf7ac54533c20) (u64 0xef22f54742509) (u64 0x6f7961ae1d9d)
+
+let p6_lseq : lseq uint64 15 =
+  assert_norm (List.Tot.length p6_list = 15);
+  Seq.seq_of_list p6_list
+
+assume
+val p6_is_pow6_lemma: unit -> Lemma (S.to_aff_point (point_eval_lseq p6_lseq) == pow_base_point 6)
+
+//-----------------------
+
+unfold
+let p7_list : list uint64 =
+  create15
+  (u64 0x92852b11abe5a) (u64 0x4f646416eae4e) (u64 0xb639adaa34214) (u64 0x18f4c410d3a43) (u64 0x10d5ba07117f)
+  (u64 0x5ccc4d5223f0c) (u64 0x5348c992c9e65) (u64 0x9dc603dd22c90) (u64 0x5fd882ef1ff18) (u64 0x740429e4bdfd)
+  (u64 0x49213a87245d0) (u64 0x1f235d735b13c) (u64 0x5a56659b7d254) (u64 0xd6f6f7b4a5eb) (u64 0xa1ea9d796daf)
+
+let p7_lseq : lseq uint64 15 =
+  assert_norm (List.Tot.length p7_list = 15);
+  Seq.seq_of_list p7_list
+
+assume
+val p7_is_pow7_lemma: unit -> Lemma (S.to_aff_point (point_eval_lseq p7_lseq) == pow_base_point 7)
+
+//-----------------------
+
+unfold
+let p8_list : list uint64 =
+  create15
+  (u64 0xd354595e8091c) (u64 0x59727a946d712) (u64 0x1ad2fd6b09d6c) (u64 0xc18040ba67527) (u64 0x94e6b56ba0ec)
+  (u64 0x80fcb21037704) (u64 0x665a87a06743f) (u64 0x1cbeb09af2bf3) (u64 0x9d72fe7feb032) (u64 0xb74df0c21371)
+  (u64 0xb17d5ffe6d714) (u64 0x1e355dee022fd) (u64 0xac21796140533) (u64 0xb639a93da6f3d) (u64 0xe15a35015997)
+
+let p8_lseq : lseq uint64 15 =
+  assert_norm (List.Tot.length p8_list = 15);
+  Seq.seq_of_list p8_list
+
+assume
+val p8_is_pow8_lemma: unit -> Lemma (S.to_aff_point (point_eval_lseq p8_lseq) == pow_base_point 8)
+
+//-----------------------
+
+unfold
+let p9_list : list uint64 =
+  create15
+  (u64 0xb9c5b6ef1f43b) (u64 0x2a7bc283fc49f) (u64 0x88e368394993f) (u64 0xed7b8a9e60d3d) (u64 0xf721d2dad6f6)
+  (u64 0xec454b7860999) (u64 0x89673b944d8e0) (u64 0x309522ce23a1a) (u64 0x5193173cc4dd9) (u64 0x9a1facd6b25a)
+  (u64 0xad69b0614f7a2) (u64 0xb8d1b10c02e19) (u64 0xbc2a2c7b66ffb) (u64 0xee4bdc91b3aa8) (u64 0xa2b275bde29d)
+
+let p9_lseq : lseq uint64 15 =
+  assert_norm (List.Tot.length p9_list = 15);
+  Seq.seq_of_list p9_list
+
+assume
+val p9_is_pow9_lemma: unit -> Lemma (S.to_aff_point (point_eval_lseq p9_lseq) == pow_base_point 9)
+
+//-----------------------
+
+unfold
+let p10_list : list uint64 =
+  create15
+  (u64 0x31ac94b24208e) (u64 0x11aeaf4ece6d) (u64 0xa413faa8d7937) (u64 0x90d8df1df29ff) (u64 0x5f8d622d2557)
+  (u64 0x592ce6949080d) (u64 0xf125a05cefe03) (u64 0x6d0aa60d51e9b) (u64 0x4f07f7c3cf9d4) (u64 0x4af6e1ccf133)
+  (u64 0xf0f95a3be72b8) (u64 0xd3f6d52e63a92) (u64 0x17d9ecbe226d1) (u64 0x6b6af333c989a) (u64 0xe625b11d9a14)
+
+let p10_lseq : lseq uint64 15 =
+  assert_norm (List.Tot.length p10_list = 15);
+  Seq.seq_of_list p10_list
+
+assume
+val p10_is_pow10_lemma: unit ->
+  Lemma (S.to_aff_point (point_eval_lseq p10_lseq) == pow_base_point 10)
+
+//-----------------------
+
+unfold
+let p11_list : list uint64 =
+  create15
+  (u64 0xd154f79d8e341) (u64 0x7cc8bb59c85ee) (u64 0xa13927fe452be) (u64 0x6e08fbee3b) (u64 0xd24d031b1185)
+  (u64 0x5c715d4620a0b) (u64 0xaa5fd2660d143) (u64 0x66bc46a0d83d0) (u64 0x2c519acec26ae) (u64 0x6c3b82462505)
+  (u64 0x8b8cbd971ab15) (u64 0xe8501868aee69) (u64 0xc54addf1d50d) (u64 0x4d8da1ea82014) (u64 0x56e000de4c56)
+
+let p11_lseq : lseq uint64 15 =
+  assert_norm (List.Tot.length p11_list = 15);
+  Seq.seq_of_list p11_list
+
+assume
+val p11_is_pow11_lemma: unit ->
+  Lemma (S.to_aff_point (point_eval_lseq p11_lseq) == pow_base_point 11)
+
+//-----------------------
+
+unfold
+let p12_list : list uint64 =
+  create15
+  (u64 0xbc3731f4e710b) (u64 0xf5fe753395cd) (u64 0x2804f4c0bc49f) (u64 0x11ae10debc618) (u64 0x4f17b524159f)
+  (u64 0xaae89f1f9385d) (u64 0x856a1901e3aea) (u64 0x2d28d08cc0cec) (u64 0x93d8d337da9b) (u64 0x5feedb5497d3)
+  (u64 0x5d06206f529e1) (u64 0x6c479715a827a) (u64 0x48a2dd96d0f48) (u64 0x3fdeb0c237630) (u64 0x1db55c9d4eaa)
+
+let p12_lseq : lseq uint64 15 =
+  assert_norm (List.Tot.length p12_list = 15);
+  Seq.seq_of_list p12_list
+
+assume
+val p12_is_pow12_lemma: unit ->
+  Lemma (S.to_aff_point (point_eval_lseq p12_lseq) == pow_base_point 12)
+
+//-----------------------
+
+unfold
+let p13_list : list uint64 =
+  create15
+  (u64 0xe0696573c7533) (u64 0x63e4658737869) (u64 0x2a11f253f4b05) (u64 0x229a7e15cdf48) (u64 0x3b9f32f54a4f)
+  (u64 0x327e4ceccc2ba) (u64 0x3e26d2be9d0df) (u64 0x82a00f70af042) (u64 0x6020d484c25d6) (u64 0xe839a854faeb)
+  (u64 0x21ded5312b490) (u64 0xf1b776c83d9ed) (u64 0x41f6a2c735d44) (u64 0x7adcc8a05f3b5) (u64 0xd926fe353140)
+
+let p13_lseq : lseq uint64 15 =
+  assert_norm (List.Tot.length p13_list = 15);
+  Seq.seq_of_list p13_list
+
+assume
+val p13_is_pow13_lemma: unit ->
+  Lemma (S.to_aff_point (point_eval_lseq p13_lseq) == pow_base_point 13)
+
+//-----------------------
+
+unfold
+let p14_list : list uint64 =
+  create15
+  (u64 0xc2b376c728ec) (u64 0x947782c52046f) (u64 0x27ba54a224d00) (u64 0x1035e99c0bf5e) (u64 0x612ca1b20e84)
+  (u64 0x789d7d062632e) (u64 0x683f45cb279ba) (u64 0x8b8fac6a007b2) (u64 0x350c84e93fa4) (u64 0x18a55aa52df)
+  (u64 0xe94da9625f527) (u64 0xd2619ce2f8a88) (u64 0x942403888b43e) (u64 0x961da5fd1dc90) (u64 0x2f1506d7e117)
+
+let p14_lseq : lseq uint64 15 =
+  assert_norm (List.Tot.length p14_list = 15);
+  Seq.seq_of_list p14_list
+
+assume
+val p14_is_pow14_lemma: unit ->
+  Lemma (S.to_aff_point (point_eval_lseq p14_lseq) == pow_base_point 14)
+
+//-----------------------
+
+unfold
+let p15_list : list uint64 =
+  create15
+  (u64 0x34deee761bce2) (u64 0xfb484324815cc) (u64 0xcd7cc675d3a1d) (u64 0xca0691e2a6447) (u64 0xbb6b7f7b8fa2)
+  (u64 0x6c53975090d10) (u64 0xa14a4124a90d2) (u64 0xbb94d4b653242) (u64 0x5074f7da14c32) (u64 0xec662837477c)
+  (u64 0xee9be37d0b9b) (u64 0x4fba9fd90713b) (u64 0xcc62c6dc14aa4) (u64 0x695bf61db25ac) (u64 0x36ba954be769)
+
+let p15_lseq : lseq uint64 15 =
+  assert_norm (List.Tot.length p15_list = 15);
+  Seq.seq_of_list p15_list
+
+assume
+val p15_is_pow15_lemma: unit ->
+  Lemma (S.to_aff_point (point_eval_lseq p15_lseq) == pow_base_point 15)
+
+//-----------------------
+
+unfold let precomp_basepoint_table_list: list uint64 =
+  normalize_term
+  FStar.List.Tot.(
+    p0_list @ p1_list @ p2_list @ p3_list
+    @ p4_list @ p5_list @ p6_list @ p7_list
+    @ p8_list @ p9_list @ p10_list @ p11_list
+    @ p12_list @ p13_list @ p14_list @ p15_list)
+
+// unfold let precomp_basepoint_table_list_l: x:list uint64{List.Tot.length x = 240} =
+//   assert_norm (List.Tot.length precomp_basepoint_table_list = 240);
+//   precomp_basepoint_table_list
+
+//-----------------------
+
+let precomp_basepoint_table_lseq : lseq uint64 240 =
+  assert_norm (List.Tot.length precomp_basepoint_table_list = 240);
+  Seq.seq_of_list precomp_basepoint_table_list
+
+val precomp_basepoint_table_lseq_lemma: unit -> Lemma
+ (sub precomp_basepoint_table_lseq 0 15 == p0_lseq /\
+  sub precomp_basepoint_table_lseq 15 15 == p1_lseq /\
+  sub precomp_basepoint_table_lseq 30 15 == p2_lseq /\
+  sub precomp_basepoint_table_lseq 45 15 == p3_lseq /\
+  sub precomp_basepoint_table_lseq 60 15 == p4_lseq /\
+  sub precomp_basepoint_table_lseq 75 15 == p5_lseq /\
+  sub precomp_basepoint_table_lseq 90 15 == p6_lseq /\
+  sub precomp_basepoint_table_lseq 105 15 == p7_lseq /\
+  sub precomp_basepoint_table_lseq 120 15 == p8_lseq /\
+  sub precomp_basepoint_table_lseq 135 15 == p9_lseq /\
+  sub precomp_basepoint_table_lseq 150 15 == p10_lseq /\
+  sub precomp_basepoint_table_lseq 165 15 == p11_lseq /\
+  sub precomp_basepoint_table_lseq 180 15 == p12_lseq /\
+  sub precomp_basepoint_table_lseq 195 15 == p13_lseq /\
+  sub precomp_basepoint_table_lseq 210 15 == p14_lseq /\
+  sub precomp_basepoint_table_lseq 225 15 == p15_lseq)
+
+let precomp_basepoint_table_lseq_lemma () =
+  Seq.elim_of_list precomp_basepoint_table_list;
+  Seq.elim_of_list p0_list;
+  eq_intro (sub precomp_basepoint_table_lseq 0 15) p0_lseq;
+  Seq.elim_of_list p1_list;
+  eq_intro (sub precomp_basepoint_table_lseq 15 15) p1_lseq;
+  Seq.elim_of_list p2_list;
+  eq_intro (sub precomp_basepoint_table_lseq 30 15) p2_lseq;
+  Seq.elim_of_list p3_list;
+  eq_intro (sub precomp_basepoint_table_lseq 45 15) p3_lseq;
+  Seq.elim_of_list p4_list;
+  eq_intro (sub precomp_basepoint_table_lseq 60 15) p4_lseq;
+  Seq.elim_of_list p5_list;
+  eq_intro (sub precomp_basepoint_table_lseq 75 15) p5_lseq;
+  Seq.elim_of_list p6_list;
+  eq_intro (sub precomp_basepoint_table_lseq 90 15) p6_lseq;
+  Seq.elim_of_list p7_list;
+  eq_intro (sub precomp_basepoint_table_lseq 105 15) p7_lseq;
+  Seq.elim_of_list p8_list;
+  eq_intro (sub precomp_basepoint_table_lseq 120 15) p8_lseq;
+  Seq.elim_of_list p9_list;
+  eq_intro (sub precomp_basepoint_table_lseq 135 15) p9_lseq;
+  Seq.elim_of_list p10_list;
+  eq_intro (sub precomp_basepoint_table_lseq 150 15) p10_lseq;
+  Seq.elim_of_list p11_list;
+  eq_intro (sub precomp_basepoint_table_lseq 165 15) p11_lseq;
+  Seq.elim_of_list p12_list;
+  eq_intro (sub precomp_basepoint_table_lseq 180 15) p12_lseq;
+  Seq.elim_of_list p13_list;
+  eq_intro (sub precomp_basepoint_table_lseq 195 15) p13_lseq;
+  Seq.elim_of_list p14_list;
+  eq_intro (sub precomp_basepoint_table_lseq 210 15) p14_lseq;
+  Seq.elim_of_list p15_list;
+  eq_intro (sub precomp_basepoint_table_lseq 225 15) p15_lseq
+
+
+unfold
+let precomp_table_inv (j:nat{j < 16}) =
+  Math.Lemmas.lemma_mult_lt_right 15 j 16;
+  Math.Lemmas.lemma_mult_le_right 15 (j + 1) 16;
+  let bj = sub precomp_basepoint_table_lseq (j * 15) 15 in
+  S.to_aff_point (point_eval_lseq bj) == pow_base_point j
+
+
+val precomp_basepoint_table_lemma_i: i:nat{i < 16} -> Lemma (precomp_table_inv i)
+let precomp_basepoint_table_lemma_i i =
+  precomp_basepoint_table_lseq_lemma ();
+  match i with
+  | 0 -> p0_is_pow0_lemma ()
+  | 1 -> p1_is_pow1_lemma ()
+  | 2 -> p2_is_pow2_lemma ()
+  | 3 -> p3_is_pow3_lemma ()
+  | 4 -> p4_is_pow4_lemma ()
+  | 5 -> p5_is_pow5_lemma ()
+  | 6 -> p6_is_pow6_lemma ()
+  | 7 -> p7_is_pow7_lemma ()
+  | 8 -> p8_is_pow8_lemma ()
+  | 9 -> p9_is_pow9_lemma ()
+  | 10 -> p10_is_pow10_lemma ()
+  | 11 -> p11_is_pow11_lemma ()
+  | 12 -> p12_is_pow12_lemma ()
+  | 13 -> p13_is_pow13_lemma ()
+  | 14 -> p14_is_pow14_lemma ()
+  | 15 -> p15_is_pow15_lemma ()
+
+val precomp_basepoint_table_lemma: unit -> Lemma (forall (i:nat{i < 16}). precomp_table_inv i)
+let precomp_basepoint_table_lemma () =
+  FStar.Classical.forall_intro precomp_basepoint_table_lemma_i
